theories/Autosubst2/syntax.v
@@ -1,4 +1,8 @@
+Require Export Lattice.All.
 Require Export unscoped.
+
+Module Type syntax_sig
+  (Export lattice : Lattice).
 
 
 
@@ -10,16 +14,8 @@ Inductive tm  : Type :=
   | tApp : ( tm   ) -> ( tm   ) -> tm 
   | tPi : ( tm   ) -> ( tm   ) -> tm 
   | tUniv : ( nat   ) -> tm 
-  | tEq : ( tm   ) -> ( tm   ) -> ( tm   ) -> tm 
-  | tJ : ( tm   ) -> ( tm   ) -> ( tm   ) -> ( tm   ) -> tm 
-  | tRefl : tm 
-  | tZero : tm 
-  | tSuc : ( tm   ) -> tm 
-  | tInd : ( tm   ) -> ( tm   ) -> ( tm   ) -> tm 
-  | tNat : tm 
-  | tSig : ( tm   ) -> ( tm   ) -> tm 
-  | tPack : ( tm   ) -> ( tm   ) -> tm 
-  | tLet : ( tm   ) -> ( tm   ) -> tm .
+  | tVoid : tm 
+  | tAbsurd : ( tm   ) -> tm .
 
 Lemma congr_tAbs  { s0 : tm   } { t0 : tm   } (H1 : s0 = t0) : tAbs  s0 = tAbs  t0 .
 Proof. congruence. Qed.
@@ -33,34 +29,10 @@ Proof. congruence. Qed.
 Lemma congr_tUniv  { s0 : nat   } { t0 : nat   } (H1 : s0 = t0) : tUniv  s0 = tUniv  t0 .
 Proof. congruence. Qed.
 
-Lemma congr_tEq  { s0 : tm   } { s1 : tm   } { s2 : tm   } { t0 : tm   } { t1 : tm   } { t2 : tm   } (H1 : s0 = t0) (H2 : s1 = t1) (H3 : s2 = t2) : tEq  s0 s1 s2 = tEq  t0 t1 t2 .
+Lemma congr_tVoid  : tVoid  = tVoid  .
 Proof. congruence. Qed.
 
-Lemma congr_tJ  { s0 : tm   } { s1 : tm   } { s2 : tm   } { s3 : tm   } { t0 : tm   } { t1 : tm   } { t2 : tm   } { t3 : tm   } (H1 : s0 = t0) (H2 : s1 = t1) (H3 : s2 = t2) (H4 : s3 = t3) : tJ  s0 s1 s2 s3 = tJ  t0 t1 t2 t3 .
-Proof. congruence. Qed.
-
-Lemma congr_tRefl  : tRefl  = tRefl  .
-Proof. congruence. Qed.
-
-Lemma congr_tZero  : tZero  = tZero  .
-Proof. congruence. Qed.
-
-Lemma congr_tSuc  { s0 : tm   } { t0 : tm   } (H1 : s0 = t0) : tSuc  s0 = tSuc  t0 .
-Proof. congruence. Qed.
-
-Lemma congr_tInd  { s0 : tm   } { s1 : tm   } { s2 : tm   } { t0 : tm   } { t1 : tm   } { t2 : tm   } (H1 : s0 = t0) (H2 : s1 = t1) (H3 : s2 = t2) : tInd  s0 s1 s2 = tInd  t0 t1 t2 .
-Proof. congruence. Qed.
-
-Lemma congr_tNat  : tNat  = tNat  .
-Proof. congruence. Qed.
-
-Lemma congr_tSig  { s0 : tm   } { s1 : tm   } { t0 : tm   } { t1 : tm   } (H1 : s0 = t0) (H2 : s1 = t1) : tSig  s0 s1 = tSig  t0 t1 .
-Proof. congruence. Qed.
-
-Lemma congr_tPack  { s0 : tm   } { s1 : tm   } { t0 : tm   } { t1 : tm   } (H1 : s0 = t0) (H2 : s1 = t1) : tPack  s0 s1 = tPack  t0 t1 .
-Proof. congruence. Qed.
-
-Lemma congr_tLet  { s0 : tm   } { s1 : tm   } { t0 : tm   } { t1 : tm   } (H1 : s0 = t0) (H2 : s1 = t1) : tLet  s0 s1 = tLet  t0 t1 .
+Lemma congr_tAbsurd  { s0 : tm   } { t0 : tm   } (H1 : s0 = t0) : tAbsurd  s0 = tAbsurd  t0 .
 Proof. congruence. Qed.
 
 Definition upRen_tm_tm   (xi : ( fin ) -> fin) : ( fin ) -> fin :=
@@ -73,16 +45,8 @@ Fixpoint ren_tm   (xitm : ( fin ) -> fin) (s : tm ) : tm  :=
     | tApp  s0 s1 => tApp  ((ren_tm xitm) s0) ((ren_tm xitm) s1)
     | tPi  s0 s1 => tPi  ((ren_tm xitm) s0) ((ren_tm (upRen_tm_tm xitm)) s1)
     | tUniv  s0 => tUniv  ((fun x => x) s0)
-    | tEq  s0 s1 s2 => tEq  ((ren_tm xitm) s0) ((ren_tm xitm) s1) ((ren_tm xitm) s2)
-    | tJ  s0 s1 s2 s3 => tJ  ((ren_tm xitm) s0) ((ren_tm xitm) s1) ((ren_tm xitm) s2) ((ren_tm xitm) s3)
-    | tRefl   => tRefl 
-    | tZero   => tZero 
-    | tSuc  s0 => tSuc  ((ren_tm xitm) s0)
-    | tInd  s0 s1 s2 => tInd  ((ren_tm xitm) s0) ((ren_tm (upRen_tm_tm (upRen_tm_tm xitm))) s1) ((ren_tm xitm) s2)
-    | tNat   => tNat 
-    | tSig  s0 s1 => tSig  ((ren_tm xitm) s0) ((ren_tm (upRen_tm_tm xitm)) s1)
-    | tPack  s0 s1 => tPack  ((ren_tm xitm) s0) ((ren_tm xitm) s1)
-    | tLet  s0 s1 => tLet  ((ren_tm xitm) s0) ((ren_tm (upRen_tm_tm (upRen_tm_tm xitm))) s1)
+    | tVoid   => tVoid 
+    | tAbsurd  s0 => tAbsurd  ((ren_tm xitm) s0)
     end.
 
 Definition up_tm_tm   (sigma : ( fin ) -> tm ) : ( fin ) -> tm  :=
@@ -95,16 +59,8 @@ Fixpoint subst_tm   (sigmatm : ( fin ) -> tm ) (s : tm ) : tm  :=
     | tApp  s0 s1 => tApp  ((subst_tm sigmatm) s0) ((subst_tm sigmatm) s1)
     | tPi  s0 s1 => tPi  ((subst_tm sigmatm) s0) ((subst_tm (up_tm_tm sigmatm)) s1)
     | tUniv  s0 => tUniv  ((fun x => x) s0)
-    | tEq  s0 s1 s2 => tEq  ((subst_tm sigmatm) s0) ((subst_tm sigmatm) s1) ((subst_tm sigmatm) s2)
-    | tJ  s0 s1 s2 s3 => tJ  ((subst_tm sigmatm) s0) ((subst_tm sigmatm) s1) ((subst_tm sigmatm) s2) ((subst_tm sigmatm) s3)
-    | tRefl   => tRefl 
-    | tZero   => tZero 
-    | tSuc  s0 => tSuc  ((subst_tm sigmatm) s0)
-    | tInd  s0 s1 s2 => tInd  ((subst_tm sigmatm) s0) ((subst_tm (up_tm_tm (up_tm_tm sigmatm))) s1) ((subst_tm sigmatm) s2)
-    | tNat   => tNat 
-    | tSig  s0 s1 => tSig  ((subst_tm sigmatm) s0) ((subst_tm (up_tm_tm sigmatm)) s1)
-    | tPack  s0 s1 => tPack  ((subst_tm sigmatm) s0) ((subst_tm sigmatm) s1)
-    | tLet  s0 s1 => tLet  ((subst_tm sigmatm) s0) ((subst_tm (up_tm_tm (up_tm_tm sigmatm))) s1)
+    | tVoid   => tVoid 
+    | tAbsurd  s0 => tAbsurd  ((subst_tm sigmatm) s0)
     end.
 
 Definition upId_tm_tm  (sigma : ( fin ) -> tm ) (Eq : forall x, sigma x = (var_tm ) x) : forall x, (up_tm_tm sigma) x = (var_tm ) x :=
@@ -119,17 +75,9 @@ Fixpoint idSubst_tm  (sigmatm : ( fin ) -> tm ) (Eqtm : forall x, sigmatm x = (v
     | tAbs  s0 => congr_tAbs ((idSubst_tm (up_tm_tm sigmatm) (upId_tm_tm (_) Eqtm)) s0)
     | tApp  s0 s1 => congr_tApp ((idSubst_tm sigmatm Eqtm) s0) ((idSubst_tm sigmatm Eqtm) s1)
     | tPi  s0 s1 => congr_tPi ((idSubst_tm sigmatm Eqtm) s0) ((idSubst_tm (up_tm_tm sigmatm) (upId_tm_tm (_) Eqtm)) s1)
-    | tUniv  s0 => congr_tUniv ((fun x => (eq_refl) x) s0)
-    | tEq  s0 s1 s2 => congr_tEq ((idSubst_tm sigmatm Eqtm) s0) ((idSubst_tm sigmatm Eqtm) s1) ((idSubst_tm sigmatm Eqtm) s2)
-    | tJ  s0 s1 s2 s3 => congr_tJ ((idSubst_tm sigmatm Eqtm) s0) ((idSubst_tm sigmatm Eqtm) s1) ((idSubst_tm sigmatm Eqtm) s2) ((idSubst_tm sigmatm Eqtm) s3)
-    | tRefl   => congr_tRefl 
-    | tZero   => congr_tZero 
-    | tSuc  s0 => congr_tSuc ((idSubst_tm sigmatm Eqtm) s0)
-    | tInd  s0 s1 s2 => congr_tInd ((idSubst_tm sigmatm Eqtm) s0) ((idSubst_tm (up_tm_tm (up_tm_tm sigmatm)) (upId_tm_tm (_) (upId_tm_tm (_) Eqtm))) s1) ((idSubst_tm sigmatm Eqtm) s2)
-    | tNat   => congr_tNat 
-    | tSig  s0 s1 => congr_tSig ((idSubst_tm sigmatm Eqtm) s0) ((idSubst_tm (up_tm_tm sigmatm) (upId_tm_tm (_) Eqtm)) s1)
-    | tPack  s0 s1 => congr_tPack ((idSubst_tm sigmatm Eqtm) s0) ((idSubst_tm sigmatm Eqtm) s1)
-    | tLet  s0 s1 => congr_tLet ((idSubst_tm sigmatm Eqtm) s0) ((idSubst_tm (up_tm_tm (up_tm_tm sigmatm)) (upId_tm_tm (_) (upId_tm_tm (_) Eqtm))) s1)
+    | tUniv  s0 => congr_tUniv eq_refl
+    | tVoid   => congr_tVoid 
+    | tAbsurd  s0 => congr_tAbsurd ((idSubst_tm sigmatm Eqtm) s0)
     end.
 
 Definition upExtRen_tm_tm   (xi : ( fin ) -> fin) (zeta : ( fin ) -> fin) (Eq : forall x, xi x = zeta x) : forall x, (upRen_tm_tm xi) x = (upRen_tm_tm zeta) x :=
@@ -144,17 +92,9 @@ Fixpoint extRen_tm   (xitm : ( fin ) -> fin) (zetatm : ( fin ) -> fin) (Eqtm : f
     | tAbs  s0 => congr_tAbs ((extRen_tm (upRen_tm_tm xitm) (upRen_tm_tm zetatm) (upExtRen_tm_tm (_) (_) Eqtm)) s0)
     | tApp  s0 s1 => congr_tApp ((extRen_tm xitm zetatm Eqtm) s0) ((extRen_tm xitm zetatm Eqtm) s1)
     | tPi  s0 s1 => congr_tPi ((extRen_tm xitm zetatm Eqtm) s0) ((extRen_tm (upRen_tm_tm xitm) (upRen_tm_tm zetatm) (upExtRen_tm_tm (_) (_) Eqtm)) s1)
-    | tUniv  s0 => congr_tUniv ((fun x => (eq_refl) x) s0)
-    | tEq  s0 s1 s2 => congr_tEq ((extRen_tm xitm zetatm Eqtm) s0) ((extRen_tm xitm zetatm Eqtm) s1) ((extRen_tm xitm zetatm Eqtm) s2)
-    | tJ  s0 s1 s2 s3 => congr_tJ ((extRen_tm xitm zetatm Eqtm) s0) ((extRen_tm xitm zetatm Eqtm) s1) ((extRen_tm xitm zetatm Eqtm) s2) ((extRen_tm xitm zetatm Eqtm) s3)
-    | tRefl   => congr_tRefl 
-    | tZero   => congr_tZero 
-    | tSuc  s0 => congr_tSuc ((extRen_tm xitm zetatm Eqtm) s0)
-    | tInd  s0 s1 s2 => congr_tInd ((extRen_tm xitm zetatm Eqtm) s0) ((extRen_tm (upRen_tm_tm (upRen_tm_tm xitm)) (upRen_tm_tm (upRen_tm_tm zetatm)) (upExtRen_tm_tm (_) (_) (upExtRen_tm_tm (_) (_) Eqtm))) s1) ((extRen_tm xitm zetatm Eqtm) s2)
-    | tNat   => congr_tNat 
-    | tSig  s0 s1 => congr_tSig ((extRen_tm xitm zetatm Eqtm) s0) ((extRen_tm (upRen_tm_tm xitm) (upRen_tm_tm zetatm) (upExtRen_tm_tm (_) (_) Eqtm)) s1)
-    | tPack  s0 s1 => congr_tPack ((extRen_tm xitm zetatm Eqtm) s0) ((extRen_tm xitm zetatm Eqtm) s1)
-    | tLet  s0 s1 => congr_tLet ((extRen_tm xitm zetatm Eqtm) s0) ((extRen_tm (upRen_tm_tm (upRen_tm_tm xitm)) (upRen_tm_tm (upRen_tm_tm zetatm)) (upExtRen_tm_tm (_) (_) (upExtRen_tm_tm (_) (_) Eqtm))) s1)
+    | tUniv  s0 => congr_tUniv eq_refl
+    | tVoid   => congr_tVoid 
+    | tAbsurd  s0 => congr_tAbsurd ((extRen_tm xitm zetatm Eqtm) s0)
     end.
 
 Definition upExt_tm_tm   (sigma : ( fin ) -> tm ) (tau : ( fin ) -> tm ) (Eq : forall x, sigma x = tau x) : forall x, (up_tm_tm sigma) x = (up_tm_tm tau) x :=
@@ -169,17 +109,9 @@ Fixpoint ext_tm   (sigmatm : ( fin ) -> tm ) (tautm : ( fin ) -> tm ) (Eqtm : fo
     | tAbs  s0 => congr_tAbs ((ext_tm (up_tm_tm sigmatm) (up_tm_tm tautm) (upExt_tm_tm (_) (_) Eqtm)) s0)
     | tApp  s0 s1 => congr_tApp ((ext_tm sigmatm tautm Eqtm) s0) ((ext_tm sigmatm tautm Eqtm) s1)
     | tPi  s0 s1 => congr_tPi ((ext_tm sigmatm tautm Eqtm) s0) ((ext_tm (up_tm_tm sigmatm) (up_tm_tm tautm) (upExt_tm_tm (_) (_) Eqtm)) s1)
-    | tUniv  s0 => congr_tUniv ((fun x => (eq_refl) x) s0)
-    | tEq  s0 s1 s2 => congr_tEq ((ext_tm sigmatm tautm Eqtm) s0) ((ext_tm sigmatm tautm Eqtm) s1) ((ext_tm sigmatm tautm Eqtm) s2)
-    | tJ  s0 s1 s2 s3 => congr_tJ ((ext_tm sigmatm tautm Eqtm) s0) ((ext_tm sigmatm tautm Eqtm) s1) ((ext_tm sigmatm tautm Eqtm) s2) ((ext_tm sigmatm tautm Eqtm) s3)
-    | tRefl   => congr_tRefl 
-    | tZero   => congr_tZero 
-    | tSuc  s0 => congr_tSuc ((ext_tm sigmatm tautm Eqtm) s0)
-    | tInd  s0 s1 s2 => congr_tInd ((ext_tm sigmatm tautm Eqtm) s0) ((ext_tm (up_tm_tm (up_tm_tm sigmatm)) (up_tm_tm (up_tm_tm tautm)) (upExt_tm_tm (_) (_) (upExt_tm_tm (_) (_) Eqtm))) s1) ((ext_tm sigmatm tautm Eqtm) s2)
-    | tNat   => congr_tNat 
-    | tSig  s0 s1 => congr_tSig ((ext_tm sigmatm tautm Eqtm) s0) ((ext_tm (up_tm_tm sigmatm) (up_tm_tm tautm) (upExt_tm_tm (_) (_) Eqtm)) s1)
-    | tPack  s0 s1 => congr_tPack ((ext_tm sigmatm tautm Eqtm) s0) ((ext_tm sigmatm tautm Eqtm) s1)
-    | tLet  s0 s1 => congr_tLet ((ext_tm sigmatm tautm Eqtm) s0) ((ext_tm (up_tm_tm (up_tm_tm sigmatm)) (up_tm_tm (up_tm_tm tautm)) (upExt_tm_tm (_) (_) (upExt_tm_tm (_) (_) Eqtm))) s1)
+    | tUniv  s0 => congr_tUniv eq_refl
+    | tVoid   => congr_tVoid 
+    | tAbsurd  s0 => congr_tAbsurd ((ext_tm sigmatm tautm Eqtm) s0)
     end.
 
 Definition up_ren_ren_tm_tm    (xi : ( fin ) -> fin) (tau : ( fin ) -> fin) (theta : ( fin ) -> fin) (Eq : forall x, ((funcomp) tau xi) x = theta x) : forall x, ((funcomp) (upRen_tm_tm tau) (upRen_tm_tm xi)) x = (upRen_tm_tm theta) x :=
@@ -191,17 +123,9 @@ Fixpoint compRenRen_tm    (xitm : ( fin ) -> fin) (zetatm : ( fin ) -> fin) (rho
     | tAbs  s0 => congr_tAbs ((compRenRen_tm (upRen_tm_tm xitm) (upRen_tm_tm zetatm) (upRen_tm_tm rhotm) (up_ren_ren (_) (_) (_) Eqtm)) s0)
     | tApp  s0 s1 => congr_tApp ((compRenRen_tm xitm zetatm rhotm Eqtm) s0) ((compRenRen_tm xitm zetatm rhotm Eqtm) s1)
     | tPi  s0 s1 => congr_tPi ((compRenRen_tm xitm zetatm rhotm Eqtm) s0) ((compRenRen_tm (upRen_tm_tm xitm) (upRen_tm_tm zetatm) (upRen_tm_tm rhotm) (up_ren_ren (_) (_) (_) Eqtm)) s1)
-    | tUniv  s0 => congr_tUniv ((fun x => (eq_refl) x) s0)
-    | tEq  s0 s1 s2 => congr_tEq ((compRenRen_tm xitm zetatm rhotm Eqtm) s0) ((compRenRen_tm xitm zetatm rhotm Eqtm) s1) ((compRenRen_tm xitm zetatm rhotm Eqtm) s2)
-    | tJ  s0 s1 s2 s3 => congr_tJ ((compRenRen_tm xitm zetatm rhotm Eqtm) s0) ((compRenRen_tm xitm zetatm rhotm Eqtm) s1) ((compRenRen_tm xitm zetatm rhotm Eqtm) s2) ((compRenRen_tm xitm zetatm rhotm Eqtm) s3)
-    | tRefl   => congr_tRefl 
-    | tZero   => congr_tZero 
-    | tSuc  s0 => congr_tSuc ((compRenRen_tm xitm zetatm rhotm Eqtm) s0)
-    | tInd  s0 s1 s2 => congr_tInd ((compRenRen_tm xitm zetatm rhotm Eqtm) s0) ((compRenRen_tm (upRen_tm_tm (upRen_tm_tm xitm)) (upRen_tm_tm (upRen_tm_tm zetatm)) (upRen_tm_tm (upRen_tm_tm rhotm)) (up_ren_ren (_) (_) (_) (up_ren_ren (_) (_) (_) Eqtm))) s1) ((compRenRen_tm xitm zetatm rhotm Eqtm) s2)
-    | tNat   => congr_tNat 
-    | tSig  s0 s1 => congr_tSig ((compRenRen_tm xitm zetatm rhotm Eqtm) s0) ((compRenRen_tm (upRen_tm_tm xitm) (upRen_tm_tm zetatm) (upRen_tm_tm rhotm) (up_ren_ren (_) (_) (_) Eqtm)) s1)
-    | tPack  s0 s1 => congr_tPack ((compRenRen_tm xitm zetatm rhotm Eqtm) s0) ((compRenRen_tm xitm zetatm rhotm Eqtm) s1)
-    | tLet  s0 s1 => congr_tLet ((compRenRen_tm xitm zetatm rhotm Eqtm) s0) ((compRenRen_tm (upRen_tm_tm (upRen_tm_tm xitm)) (upRen_tm_tm (upRen_tm_tm zetatm)) (upRen_tm_tm (upRen_tm_tm rhotm)) (up_ren_ren (_) (_) (_) (up_ren_ren (_) (_) (_) Eqtm))) s1)
+    | tUniv  s0 => congr_tUniv eq_refl
+    | tVoid   => congr_tVoid 
+    | tAbsurd  s0 => congr_tAbsurd ((compRenRen_tm xitm zetatm rhotm Eqtm) s0)
     end.
 
 Definition up_ren_subst_tm_tm    (xi : ( fin ) -> fin) (tau : ( fin ) -> tm ) (theta : ( fin ) -> tm ) (Eq : forall x, ((funcomp) tau xi) x = theta x) : forall x, ((funcomp) (up_tm_tm tau) (upRen_tm_tm xi)) x = (up_tm_tm theta) x :=
@@ -216,17 +140,9 @@ Fixpoint compRenSubst_tm    (xitm : ( fin ) -> fin) (tautm : ( fin ) -> tm ) (th
     | tAbs  s0 => congr_tAbs ((compRenSubst_tm (upRen_tm_tm xitm) (up_tm_tm tautm) (up_tm_tm thetatm) (up_ren_subst_tm_tm (_) (_) (_) Eqtm)) s0)
     | tApp  s0 s1 => congr_tApp ((compRenSubst_tm xitm tautm thetatm Eqtm) s0) ((compRenSubst_tm xitm tautm thetatm Eqtm) s1)
     | tPi  s0 s1 => congr_tPi ((compRenSubst_tm xitm tautm thetatm Eqtm) s0) ((compRenSubst_tm (upRen_tm_tm xitm) (up_tm_tm tautm) (up_tm_tm thetatm) (up_ren_subst_tm_tm (_) (_) (_) Eqtm)) s1)
-    | tUniv  s0 => congr_tUniv ((fun x => (eq_refl) x) s0)
-    | tEq  s0 s1 s2 => congr_tEq ((compRenSubst_tm xitm tautm thetatm Eqtm) s0) ((compRenSubst_tm xitm tautm thetatm Eqtm) s1) ((compRenSubst_tm xitm tautm thetatm Eqtm) s2)
-    | tJ  s0 s1 s2 s3 => congr_tJ ((compRenSubst_tm xitm tautm thetatm Eqtm) s0) ((compRenSubst_tm xitm tautm thetatm Eqtm) s1) ((compRenSubst_tm xitm tautm thetatm Eqtm) s2) ((compRenSubst_tm xitm tautm thetatm Eqtm) s3)
-    | tRefl   => congr_tRefl 
-    | tZero   => congr_tZero 
-    | tSuc  s0 => congr_tSuc ((compRenSubst_tm xitm tautm thetatm Eqtm) s0)
-    | tInd  s0 s1 s2 => congr_tInd ((compRenSubst_tm xitm tautm thetatm Eqtm) s0) ((compRenSubst_tm (upRen_tm_tm (upRen_tm_tm xitm)) (up_tm_tm (up_tm_tm tautm)) (up_tm_tm (up_tm_tm thetatm)) (up_ren_subst_tm_tm (_) (_) (_) (up_ren_subst_tm_tm (_) (_) (_) Eqtm))) s1) ((compRenSubst_tm xitm tautm thetatm Eqtm) s2)
-    | tNat   => congr_tNat 
-    | tSig  s0 s1 => congr_tSig ((compRenSubst_tm xitm tautm thetatm Eqtm) s0) ((compRenSubst_tm (upRen_tm_tm xitm) (up_tm_tm tautm) (up_tm_tm thetatm) (up_ren_subst_tm_tm (_) (_) (_) Eqtm)) s1)
-    | tPack  s0 s1 => congr_tPack ((compRenSubst_tm xitm tautm thetatm Eqtm) s0) ((compRenSubst_tm xitm tautm thetatm Eqtm) s1)
-    | tLet  s0 s1 => congr_tLet ((compRenSubst_tm xitm tautm thetatm Eqtm) s0) ((compRenSubst_tm (upRen_tm_tm (upRen_tm_tm xitm)) (up_tm_tm (up_tm_tm tautm)) (up_tm_tm (up_tm_tm thetatm)) (up_ren_subst_tm_tm (_) (_) (_) (up_ren_subst_tm_tm (_) (_) (_) Eqtm))) s1)
+    | tUniv  s0 => congr_tUniv eq_refl
+    | tVoid   => congr_tVoid 
+    | tAbsurd  s0 => congr_tAbsurd ((compRenSubst_tm xitm tautm thetatm Eqtm) s0)
     end.
 
 Definition up_subst_ren_tm_tm    (sigma : ( fin ) -> tm ) (zetatm : ( fin ) -> fin) (theta : ( fin ) -> tm ) (Eq : forall x, ((funcomp) (ren_tm zetatm) sigma) x = theta x) : forall x, ((funcomp) (ren_tm (upRen_tm_tm zetatm)) (up_tm_tm sigma)) x = (up_tm_tm theta) x :=
@@ -241,17 +157,9 @@ Fixpoint compSubstRen_tm    (sigmatm : ( fin ) -> tm ) (zetatm : ( fin ) -> fin)
     | tAbs  s0 => congr_tAbs ((compSubstRen_tm (up_tm_tm sigmatm) (upRen_tm_tm zetatm) (up_tm_tm thetatm) (up_subst_ren_tm_tm (_) (_) (_) Eqtm)) s0)
     | tApp  s0 s1 => congr_tApp ((compSubstRen_tm sigmatm zetatm thetatm Eqtm) s0) ((compSubstRen_tm sigmatm zetatm thetatm Eqtm) s1)
     | tPi  s0 s1 => congr_tPi ((compSubstRen_tm sigmatm zetatm thetatm Eqtm) s0) ((compSubstRen_tm (up_tm_tm sigmatm) (upRen_tm_tm zetatm) (up_tm_tm thetatm) (up_subst_ren_tm_tm (_) (_) (_) Eqtm)) s1)
-    | tUniv  s0 => congr_tUniv ((fun x => (eq_refl) x) s0)
-    | tEq  s0 s1 s2 => congr_tEq ((compSubstRen_tm sigmatm zetatm thetatm Eqtm) s0) ((compSubstRen_tm sigmatm zetatm thetatm Eqtm) s1) ((compSubstRen_tm sigmatm zetatm thetatm Eqtm) s2)
-    | tJ  s0 s1 s2 s3 => congr_tJ ((compSubstRen_tm sigmatm zetatm thetatm Eqtm) s0) ((compSubstRen_tm sigmatm zetatm thetatm Eqtm) s1) ((compSubstRen_tm sigmatm zetatm thetatm Eqtm) s2) ((compSubstRen_tm sigmatm zetatm thetatm Eqtm) s3)
-    | tRefl   => congr_tRefl 
-    | tZero   => congr_tZero 
-    | tSuc  s0 => congr_tSuc ((compSubstRen_tm sigmatm zetatm thetatm Eqtm) s0)
-    | tInd  s0 s1 s2 => congr_tInd ((compSubstRen_tm sigmatm zetatm thetatm Eqtm) s0) ((compSubstRen_tm (up_tm_tm (up_tm_tm sigmatm)) (upRen_tm_tm (upRen_tm_tm zetatm)) (up_tm_tm (up_tm_tm thetatm)) (up_subst_ren_tm_tm (_) (_) (_) (up_subst_ren_tm_tm (_) (_) (_) Eqtm))) s1) ((compSubstRen_tm sigmatm zetatm thetatm Eqtm) s2)
-    | tNat   => congr_tNat 
-    | tSig  s0 s1 => congr_tSig ((compSubstRen_tm sigmatm zetatm thetatm Eqtm) s0) ((compSubstRen_tm (up_tm_tm sigmatm) (upRen_tm_tm zetatm) (up_tm_tm thetatm) (up_subst_ren_tm_tm (_) (_) (_) Eqtm)) s1)
-    | tPack  s0 s1 => congr_tPack ((compSubstRen_tm sigmatm zetatm thetatm Eqtm) s0) ((compSubstRen_tm sigmatm zetatm thetatm Eqtm) s1)
-    | tLet  s0 s1 => congr_tLet ((compSubstRen_tm sigmatm zetatm thetatm Eqtm) s0) ((compSubstRen_tm (up_tm_tm (up_tm_tm sigmatm)) (upRen_tm_tm (upRen_tm_tm zetatm)) (up_tm_tm (up_tm_tm thetatm)) (up_subst_ren_tm_tm (_) (_) (_) (up_subst_ren_tm_tm (_) (_) (_) Eqtm))) s1)
+    | tUniv  s0 => congr_tUniv eq_refl
+    | tVoid   => congr_tVoid 
+    | tAbsurd  s0 => congr_tAbsurd ((compSubstRen_tm sigmatm zetatm thetatm Eqtm) s0)
     end.
 
 Definition up_subst_subst_tm_tm    (sigma : ( fin ) -> tm ) (tautm : ( fin ) -> tm ) (theta : ( fin ) -> tm ) (Eq : forall x, ((funcomp) (subst_tm tautm) sigma) x = theta x) : forall x, ((funcomp) (subst_tm (up_tm_tm tautm)) (up_tm_tm sigma)) x = (up_tm_tm theta) x :=
@@ -266,17 +174,9 @@ Fixpoint compSubstSubst_tm    (sigmatm : ( fin ) -> tm ) (tautm : ( fin ) -> tm 
     | tAbs  s0 => congr_tAbs ((compSubstSubst_tm (up_tm_tm sigmatm) (up_tm_tm tautm) (up_tm_tm thetatm) (up_subst_subst_tm_tm (_) (_) (_) Eqtm)) s0)
     | tApp  s0 s1 => congr_tApp ((compSubstSubst_tm sigmatm tautm thetatm Eqtm) s0) ((compSubstSubst_tm sigmatm tautm thetatm Eqtm) s1)
     | tPi  s0 s1 => congr_tPi ((compSubstSubst_tm sigmatm tautm thetatm Eqtm) s0) ((compSubstSubst_tm (up_tm_tm sigmatm) (up_tm_tm tautm) (up_tm_tm thetatm) (up_subst_subst_tm_tm (_) (_) (_) Eqtm)) s1)
-    | tUniv  s0 => congr_tUniv ((fun x => (eq_refl) x) s0)
-    | tEq  s0 s1 s2 => congr_tEq ((compSubstSubst_tm sigmatm tautm thetatm Eqtm) s0) ((compSubstSubst_tm sigmatm tautm thetatm Eqtm) s1) ((compSubstSubst_tm sigmatm tautm thetatm Eqtm) s2)
-    | tJ  s0 s1 s2 s3 => congr_tJ ((compSubstSubst_tm sigmatm tautm thetatm Eqtm) s0) ((compSubstSubst_tm sigmatm tautm thetatm Eqtm) s1) ((compSubstSubst_tm sigmatm tautm thetatm Eqtm) s2) ((compSubstSubst_tm sigmatm tautm thetatm Eqtm) s3)
-    | tRefl   => congr_tRefl 
-    | tZero   => congr_tZero 
-    | tSuc  s0 => congr_tSuc ((compSubstSubst_tm sigmatm tautm thetatm Eqtm) s0)
-    | tInd  s0 s1 s2 => congr_tInd ((compSubstSubst_tm sigmatm tautm thetatm Eqtm) s0) ((compSubstSubst_tm (up_tm_tm (up_tm_tm sigmatm)) (up_tm_tm (up_tm_tm tautm)) (up_tm_tm (up_tm_tm thetatm)) (up_subst_subst_tm_tm (_) (_) (_) (up_subst_subst_tm_tm (_) (_) (_) Eqtm))) s1) ((compSubstSubst_tm sigmatm tautm thetatm Eqtm) s2)
-    | tNat   => congr_tNat 
-    | tSig  s0 s1 => congr_tSig ((compSubstSubst_tm sigmatm tautm thetatm Eqtm) s0) ((compSubstSubst_tm (up_tm_tm sigmatm) (up_tm_tm tautm) (up_tm_tm thetatm) (up_subst_subst_tm_tm (_) (_) (_) Eqtm)) s1)
-    | tPack  s0 s1 => congr_tPack ((compSubstSubst_tm sigmatm tautm thetatm Eqtm) s0) ((compSubstSubst_tm sigmatm tautm thetatm Eqtm) s1)
-    | tLet  s0 s1 => congr_tLet ((compSubstSubst_tm sigmatm tautm thetatm Eqtm) s0) ((compSubstSubst_tm (up_tm_tm (up_tm_tm sigmatm)) (up_tm_tm (up_tm_tm tautm)) (up_tm_tm (up_tm_tm thetatm)) (up_subst_subst_tm_tm (_) (_) (_) (up_subst_subst_tm_tm (_) (_) (_) Eqtm))) s1)
+    | tUniv  s0 => congr_tUniv eq_refl
+    | tVoid   => congr_tVoid 
+    | tAbsurd  s0 => congr_tAbsurd ((compSubstSubst_tm sigmatm tautm thetatm Eqtm) s0)
     end.
 
 Definition rinstInst_up_tm_tm   (xi : ( fin ) -> fin) (sigma : ( fin ) -> tm ) (Eq : forall x, ((funcomp) (var_tm ) xi) x = sigma x) : forall x, ((funcomp) (var_tm ) (upRen_tm_tm xi)) x = (up_tm_tm sigma) x :=
@@ -291,17 +191,9 @@ Fixpoint rinst_inst_tm   (xitm : ( fin ) -> fin) (sigmatm : ( fin ) -> tm ) (Eqt
     | tAbs  s0 => congr_tAbs ((rinst_inst_tm (upRen_tm_tm xitm) (up_tm_tm sigmatm) (rinstInst_up_tm_tm (_) (_) Eqtm)) s0)
     | tApp  s0 s1 => congr_tApp ((rinst_inst_tm xitm sigmatm Eqtm) s0) ((rinst_inst_tm xitm sigmatm Eqtm) s1)
     | tPi  s0 s1 => congr_tPi ((rinst_inst_tm xitm sigmatm Eqtm) s0) ((rinst_inst_tm (upRen_tm_tm xitm) (up_tm_tm sigmatm) (rinstInst_up_tm_tm (_) (_) Eqtm)) s1)
-    | tUniv  s0 => congr_tUniv ((fun x => (eq_refl) x) s0)
-    | tEq  s0 s1 s2 => congr_tEq ((rinst_inst_tm xitm sigmatm Eqtm) s0) ((rinst_inst_tm xitm sigmatm Eqtm) s1) ((rinst_inst_tm xitm sigmatm Eqtm) s2)
-    | tJ  s0 s1 s2 s3 => congr_tJ ((rinst_inst_tm xitm sigmatm Eqtm) s0) ((rinst_inst_tm xitm sigmatm Eqtm) s1) ((rinst_inst_tm xitm sigmatm Eqtm) s2) ((rinst_inst_tm xitm sigmatm Eqtm) s3)
-    | tRefl   => congr_tRefl 
-    | tZero   => congr_tZero 
-    | tSuc  s0 => congr_tSuc ((rinst_inst_tm xitm sigmatm Eqtm) s0)
-    | tInd  s0 s1 s2 => congr_tInd ((rinst_inst_tm xitm sigmatm Eqtm) s0) ((rinst_inst_tm (upRen_tm_tm (upRen_tm_tm xitm)) (up_tm_tm (up_tm_tm sigmatm)) (rinstInst_up_tm_tm (_) (_) (rinstInst_up_tm_tm (_) (_) Eqtm))) s1) ((rinst_inst_tm xitm sigmatm Eqtm) s2)
-    | tNat   => congr_tNat 
-    | tSig  s0 s1 => congr_tSig ((rinst_inst_tm xitm sigmatm Eqtm) s0) ((rinst_inst_tm (upRen_tm_tm xitm) (up_tm_tm sigmatm) (rinstInst_up_tm_tm (_) (_) Eqtm)) s1)
-    | tPack  s0 s1 => congr_tPack ((rinst_inst_tm xitm sigmatm Eqtm) s0) ((rinst_inst_tm xitm sigmatm Eqtm) s1)
-    | tLet  s0 s1 => congr_tLet ((rinst_inst_tm xitm sigmatm Eqtm) s0) ((rinst_inst_tm (upRen_tm_tm (upRen_tm_tm xitm)) (up_tm_tm (up_tm_tm sigmatm)) (rinstInst_up_tm_tm (_) (_) (rinstInst_up_tm_tm (_) (_) Eqtm))) s1)
+    | tUniv  s0 => congr_tUniv eq_refl
+    | tVoid   => congr_tVoid 
+    | tAbsurd  s0 => congr_tAbsurd ((rinst_inst_tm xitm sigmatm Eqtm) s0)
     end.
 
 Lemma rinstInst_tm   (xitm : ( fin ) -> fin) : ren_tm xitm = subst_tm ((funcomp) (var_tm ) xitm) .
@@ -344,22 +236,6 @@ Lemma renRen'_tm    (xitm : ( fin ) -> fin) (zetatm : ( fin ) -> fin) : (funcomp
 Proof. exact ((FunctionalExtensionality.functional_extensionality _ _ ) (fun n => renRen_tm xitm zetatm n)). Qed.
 
 End tm.
-
-
-
-
-
-
-
-
-
-
-
-
-
-
-
-
 
 
 
@@ -421,3 +297,4 @@ Ltac substify := auto_unfold; try repeat (erewrite rinstInst_tm).
 
 Ltac renamify := auto_unfold; try repeat (erewrite <- rinstInst_tm).
 
+End syntax_sig.
