theories/join.v
@@ -40,72 +40,12 @@ Inductive Par : tm -> tm -> Prop :=
   (b0 ⇒ b1) ->
   (* ---------------------------- *)
   (tApp (tAbs a) b0) ⇒ (a0 [b1..])
-| P_Zero :
-  (* ------- *)
-  tZero ⇒ tZero
-| P_Suc a b :
+| P_Void :
+  tVoid ⇒ tVoid
+| P_Absurd a b :
   a ⇒ b ->
   (* ---------- *)
-  tSuc a ⇒ tSuc b
-| P_Ind a0 a1 b0 b1 c0 c1:
-  a0 ⇒ a1 ->
-  b0 ⇒ b1 ->
-  c0 ⇒ c1 ->
-  (* ---------- *)
-  tInd a0 b0 c0 ⇒ tInd a1 b1 c1
-| P_IndZero a0 a1 b:
-  a0 ⇒ a1 ->
-  (* ---------- *)
-  tInd a0 b tZero ⇒ a1
-| P_IndSuc a0 a1 b0 b1 c0 c1 :
-  a0 ⇒ a1 ->
-  b0 ⇒ b1 ->
-  c0 ⇒ c1 ->
-  (* ---------------------  *)
-  tInd a0 b0 (tSuc c0) ⇒ b1 [(tInd a1 b1 c1) .: c1  ..]
-| P_Nat :
-  (* ---------- *)
-  tNat ⇒ tNat
-| P_Refl :
-  (* ---------- *)
-  tRefl ⇒ tRefl
-| P_Eq a0 b0 A0 a1 b1 A1 :
-  (a0 ⇒ a1) ->
-  (b0 ⇒ b1) ->
-  (A0 ⇒ A1) ->
-  (* ---------- *)
-  (tEq a0 b0 A0) ⇒ (tEq a1 b1 A1)
-| P_J t0 a0 b0 p0 t1 a1 b1 p1 :
-  (t0 ⇒ t1) ->
-  (a0 ⇒ a1) ->
-  (b0 ⇒ b1) ->
-  (p0 ⇒ p1) ->
-  (* ---------- *)
-  (tJ t0 a0 b0 p0) ⇒ (tJ t1 a1 b1 p1)
-| P_JRefl t0 a b t1 :
-  (t0 ⇒ t1) ->
-  (* ---------- *)
-  (tJ t0 a b tRefl) ⇒ t1
-| P_Sig A0 A1 B0 B1 :
-  (A0 ⇒ A1) ->
-  (B0 ⇒ B1) ->
-  (* --------------------- *)
-  tSig A0 B0 ⇒ tSig A1 B1
-| P_Pack a0 a1 b0 b1 :
-  (a0 ⇒ a1) ->
-  (b0 ⇒ b1) ->
-  (* ------------------------- *)
-  (tPack a0 b0) ⇒ (tPack a1 b1)
-| P_Let a0 b0 a1 b1 :
-  a0 ⇒ a1 ->
-  b0 ⇒ b1 ->
-  (* --------------------- *)
-  tLet a0 b0 ⇒ tLet a1 b1
-| P_LetPack a0 b0 c0 a1 b1 c1 :
-  a0 ⇒ a1 ->
-  b0 ⇒ b1 ->
-  c0 ⇒ c1 ->
-  tLet (tPack a0 b0) c0 ⇒ c1[b1 .: a1 ..]
+  tAbsurd a ⇒ tAbsurd b
 where "A ⇒ B" := (Par A B).
 #[export]Hint Constructors Par : par.
 
@@ -142,22 +82,22 @@ Lemma P_AppAbs' a a0 b0 b b1 :
   (tApp (tAbs a) b0) ⇒ b.
 Proof. hauto lq:on use:P_AppAbs. Qed.
 
-Lemma P_IndSuc' a0 a1 b0 b1 c0 c1 t :
-  t = b1 [(tInd a1 b1 c1) .: c1 ..] ->
-  a0 ⇒ a1 ->
-  b0 ⇒ b1 ->
-  c0 ⇒ c1 ->
-  (* ---------------------  *)
-  tInd a0 b0 (tSuc c0) ⇒ t.
-Proof. move => > ->. apply P_IndSuc. Qed.
+(* Lemma P_IndSuc' a0 a1 b0 b1 c0 c1 t : *)
+(*   t = b1 [(tInd a1 b1 c1) .: c1 ..] -> *)
+(*   a0 ⇒ a1 -> *)
+(*   b0 ⇒ b1 -> *)
+(*   c0 ⇒ c1 -> *)
+(*   (* ---------------------  *) *)
+(*   tInd a0 b0 (tSuc c0) ⇒ t. *)
+(* Proof. move => > ->. apply P_IndSuc. Qed. *)
 
-Lemma P_LetPack' a0 b0 c0 a1 b1 c1 t :
-  t = c1[b1 .: a1 ..] ->
-  a0 ⇒ a1 ->
-  b0 ⇒ b1 ->
-  c0 ⇒ c1 ->
-  tLet (tPack a0 b0) c0 ⇒ t.
-Proof. move => > ->. apply P_LetPack. Qed.
+(* Lemma P_LetPack' a0 b0 c0 a1 b1 c1 t : *)
+(*   t = c1[b1 .: a1 ..] -> *)
+(*   a0 ⇒ a1 -> *)
+(*   b0 ⇒ b1 -> *)
+(*   c0 ⇒ c1 -> *)
+(*   tLet (tPack a0 b0) c0 ⇒ t. *)
+(* Proof. move => > ->. apply P_LetPack. Qed. *)
 
 (* ------------------------------------------------------------ *)
 
@@ -171,10 +111,10 @@ Proof.
   elim : a b / h => /=; eauto with par.
   - move => *.
     apply : P_AppAbs'; eauto. by asimpl.
-  - move => *.
-    apply : P_IndSuc'; eauto; by asimpl.
-  - move => *.
-    apply : P_LetPack'; eauto; by asimpl.
+  (* - move => *. *)
+  (*   apply : P_IndSuc'; eauto; by asimpl. *)
+  (* - move => *. *)
+  (*   apply : P_LetPack'; eauto; by asimpl. *)
 Qed.
 
 Lemma Pars_renaming a b (ξ : fin -> fin) :
@@ -225,19 +165,19 @@ Proof.
   - move => a a0 b0 b1 h0 ih0 h1 ih1 σ0 σ h /=.
     apply P_AppAbs' with (a0 := a0 [up_tm_tm σ]) (b1 := b1 [σ]).
     by asimpl. hauto l:on unfold:Par_m use:Par_renaming inv:nat. eauto.
-  - qauto db:par use:(Par_morphing_lift_n 2).
-  - move => a0 a1 b0 b1 c0 c1 ha iha hb ihb hc ihc σ0 σ1 hσ /=.
-    apply P_IndSuc' with
-      (b1 := b1[up_tm_tm_n 2 σ1]) (a1 := a1[σ1]) (c1 := c1[σ1]);
-      eauto => /=. by asimpl.
-    sfirstorder use:(Par_morphing_lift_n 2).
-  - hauto lq:on db:par use:(Par_morphing_lift_n 1).
-  - qauto db:par use:(Par_morphing_lift_n 1).
-  - qauto l:on ctrs:Par use:(Par_morphing_lift_n 2).
-  - move => a0 b0 c0 a1 b1 c1 ha iha hb ihb hc ihc σ0 σ1 hσ /=.
-    apply P_LetPack' with (a1 := a1[σ1]) (b1 := b1[σ1]) (c1 := c1[up_tm_tm (up_tm_tm σ1)]); eauto.
-    by asimpl.
-    sfirstorder use:(Par_morphing_lift_n 2).
+  (* - qauto db:par use:(Par_morphing_lift_n 2). *)
+  (* - move => a0 a1 b0 b1 c0 c1 ha iha hb ihb hc ihc σ0 σ1 hσ /=. *)
+  (*   apply P_IndSuc' with *)
+  (*     (b1 := b1[up_tm_tm_n 2 σ1]) (a1 := a1[σ1]) (c1 := c1[σ1]); *)
+  (*     eauto => /=. by asimpl. *)
+  (*   sfirstorder use:(Par_morphing_lift_n 2). *)
+  (* - hauto lq:on db:par use:(Par_morphing_lift_n 1). *)
+  (* - qauto db:par use:(Par_morphing_lift_n 1). *)
+  (* - qauto l:on ctrs:Par use:(Par_morphing_lift_n 2). *)
+  (* - move => a0 b0 c0 a1 b1 c1 ha iha hb ihb hc ihc σ0 σ1 hσ /=. *)
+  (*   apply P_LetPack' with (a1 := a1[σ1]) (b1 := b1[σ1]) (c1 := c1[up_tm_tm (up_tm_tm σ1)]); eauto. *)
+  (*   by asimpl. *)
+  (*   sfirstorder use:(Par_morphing_lift_n 2). *)
 Qed.
 
 Lemma Par_morphing_star a0 a1 (h : a0 ⇒* a1) (σ0 σ1 : fin -> tm) :
@@ -391,13 +331,13 @@ Proof.
   elim : T C / h; hecrush inv:Par ctrs:Par, rtc.
 Qed.
 
-Lemma Pars_eq_inv a b A C (h : (tEq a b A) ⇒* C) :
-  exists a0 b0 A0, C = tEq a0 b0 A0 /\ a ⇒* a0 /\ b ⇒* b0 /\ A ⇒* A0.
-Proof.
-  move E : (tEq a b A) h => T h.
-  move : a b A E.
-  elim : T C / h; hecrush inv:Par ctrs:Par, rtc.
-Qed.
+(* Lemma Pars_eq_inv a b A C (h : (tEq a b A) ⇒* C) : *)
+(*   exists a0 b0 A0, C = tEq a0 b0 A0 /\ a ⇒* a0 /\ b ⇒* b0 /\ A ⇒* A0. *)
+(* Proof. *)
+(*   move E : (tEq a b A) h => T h. *)
+(*   move : a b A E. *)
+(*   elim : T C / h; hecrush inv:Par ctrs:Par, rtc. *)
+(* Qed. *)
 
 Lemma Pars_univ_inv i A (h : (tUniv i) ⇒* A) :
   A = tUniv i.
@@ -407,85 +347,84 @@ Proof.
   elim : A0 A / h; hauto q:on rew:off ctrs:rtc, Par inv:Par.
 Qed.
 
-Lemma Pars_sig_inv A B C (h : tSig A B ⇒* C) :
-  exists A0 B0, C = tSig A0 B0 /\ (A ⇒* A0) /\ (B ⇒* B0).
-Proof.
-  move E : (tSig A B) h => T h.
-  move : A B E.
-  elim : T C / h; hecrush inv:Par ctrs:Par, rtc.
-Qed.
+(* Lemma Pars_sig_inv A B C (h : tSig A B ⇒* C) : *)
+(*   exists A0 B0, C = tSig A0 B0 /\ (A ⇒* A0) /\ (B ⇒* B0). *)
+(* Proof. *)
+(*   move E : (tSig A B) h => T h. *)
+(*   move : A B E. *)
+(*   elim : T C / h; hecrush inv:Par ctrs:Par, rtc. *)
+(* Qed. *)
 
 Lemma Coherent_univ_inj i j (h : Coherent (tUniv i) (tUniv j)) : i = j.
 Proof. hauto lq:on rew:off inv:rtc use:Pars_univ_inv. Qed.
 
-
 (* ------------------------------------------------------------ *)
 
 
-Lemma P_IndZero_star a b c :
-  (c ⇒* tZero) ->
-  (tInd a b c  ⇒* a).
-Proof.
-  move E : tZero => v h.
-  move : E.
-  elim : c v / h.
-  - move => *. subst.
-    apply rtc_once. apply P_IndZero. apply Par_refl.
-  - move => c c0 c1 h0 h1 h2 ?; subst.
-    move /(_ eq_refl) in h2.
-    apply : rtc_transitive; eauto.
-    hauto lq:on use:@rtc_once,Par_refl ctrs:Par.
-Qed.
+(* Lemma P_IndZero_star a b c : *)
+(*   (c ⇒* tZero) -> *)
+(*   (tInd a b c  ⇒* a). *)
+(* Proof. *)
+(*   move E : tZero => v h. *)
+(*   move : E. *)
+(*   elim : c v / h. *)
+(*   - move => *. subst. *)
+(*     apply rtc_once. apply P_IndZero. apply Par_refl. *)
+(*   - move => c c0 c1 h0 h1 h2 ?; subst. *)
+(*     move /(_ eq_refl) in h2. *)
+(*     apply : rtc_transitive; eauto. *)
+(*     hauto lq:on use:@rtc_once,Par_refl ctrs:Par. *)
+(* Qed. *)
 
-Lemma P_IndSuc_star a b c c0 :
-  (c ⇒* tSuc c0) ->
-  (tInd a b c  ⇒* b[(tInd a b c0) .: c0 ..]).
-Proof.
-  move E : (tSuc c0) => v h.
-  move : E.  elim : c v /h.
-  - move=> > <- *.
-    apply rtc_once. apply P_IndSuc; apply Par_refl.
-  - move => c1 c2 c3 h0 h1 ih ?. subst.
-    move /(_ eq_refl) : ih.
-    apply rtc_l.
-    hauto lq:on use:Par_refl ctrs:Par.
-Qed.
+(* Lemma P_IndSuc_star a b c c0 : *)
+(*   (c ⇒* tSuc c0) -> *)
+(*   (tInd a b c  ⇒* b[(tInd a b c0) .: c0 ..]). *)
+(* Proof. *)
+(*   move E : (tSuc c0) => v h. *)
+(*   move : E.  elim : c v /h. *)
+(*   - move=> > <- *. *)
+(*     apply rtc_once. apply P_IndSuc; apply Par_refl. *)
+(*   - move => c1 c2 c3 h0 h1 ih ?. subst. *)
+(*     move /(_ eq_refl) : ih. *)
+(*     apply rtc_l. *)
+(*     hauto lq:on use:Par_refl ctrs:Par. *)
+(* Qed. *)
 
-Lemma P_IndSuc_star' a b c c0 t :
-  b[(tInd a b c0) .: c0 ..] = t ->
-  (c ⇒* tSuc c0) ->
-  (tInd a b c  ⇒* t).
-Proof. move => > <-. apply P_IndSuc_star. Qed.
+(* Lemma P_IndSuc_star' a b c c0 t : *)
+(*   b[(tInd a b c0) .: c0 ..] = t -> *)
+(*   (c ⇒* tSuc c0) -> *)
+(*   (tInd a b c  ⇒* t). *)
+(* Proof. move => > <-. apply P_IndSuc_star. Qed. *)
 
-Lemma P_JRefl_star t a b p :
-  (p ⇒* tRefl)  ->
-  ((tJ t a b p) ⇒* t).
-Proof.
-  move E : tRefl => v h.
-  move : E.
-  elim : p v / h.
-  - move => *. subst.
-    apply rtc_once. apply P_JRefl. apply Par_refl.
-  - move => x y z h0 h1 ih ?; subst.
-    move /(_ ltac:(done)) in ih.
-    apply : rtc_l; eauto.
-    apply P_J; sfirstorder use:Par_refl.
-Qed.
+(* Lemma P_JRefl_star t a b p : *)
+(*   (p ⇒* tRefl)  -> *)
+(*   ((tJ t a b p) ⇒* t). *)
+(* Proof. *)
+(*   move E : tRefl => v h. *)
+(*   move : E. *)
+(*   elim : p v / h. *)
+(*   - move => *. subst. *)
+(*     apply rtc_once. apply P_JRefl. apply Par_refl. *)
+(*   - move => x y z h0 h1 ih ?; subst. *)
+(*     move /(_ ltac:(done)) in ih. *)
+(*     apply : rtc_l; eauto. *)
+(*     apply P_J; sfirstorder use:Par_refl. *)
+(* Qed. *)
 
-Lemma P_LetPack_star t a b c :
-  t ⇒* tPack a b ->
-  tLet t c ⇒* c[b .: a ..].
-Proof.
-  move E : (tPack a b) => v h.
-  move : a b c E.
-  elim:t v/h.
-  - move => *. subst.
-    apply rtc_once. apply P_LetPack; apply Par_refl.
-  - move => t0 t ? h0 h1 ih a b c ?. subst.
-    specialize ih with (1 := eq_refl).
-    apply : rtc_l; eauto.
-    apply P_Let=>//. apply Par_refl.
-Qed.
+(* Lemma P_LetPack_star t a b c : *)
+(*   t ⇒* tPack a b -> *)
+(*   tLet t c ⇒* c[b .: a ..]. *)
+(* Proof. *)
+(*   move E : (tPack a b) => v h. *)
+(*   move : a b c E. *)
+(*   elim:t v/h. *)
+(*   - move => *. subst. *)
+(*     apply rtc_once. apply P_LetPack; apply Par_refl. *)
+(*   - move => t0 t ? h0 h1 ih a b c ?. subst. *)
+(*     specialize ih with (1 := eq_refl). *)
+(*     apply : rtc_l; eauto. *)
+(*     apply P_Let=>//. apply Par_refl. *)
+(* Qed. *)
 
 (* ------------------------------------------------------------ *)
 
@@ -508,20 +447,22 @@ Function tstar (a : tm) :=
   | tAbs a => tAbs (tstar a)
   | tApp (tAbs a) b =>  (tstar a) [(tstar b)..]
   | tApp a b => tApp (tstar a) (tstar b)
-  | tZero => tZero
-  | tSuc a => tSuc (tstar a)
-  | tInd a b tZero => tstar a
-  | tInd a b (tSuc c) => (tstar b) [(tInd (tstar a) (tstar b) (tstar c)) .: (tstar c)  .. ]
-  | tInd a b c => tInd (tstar a) (tstar b) (tstar c)
-  | tNat => tNat
-  | tRefl => tRefl
-  | tEq a b A => tEq (tstar a) (tstar b) (tstar A)
-  | tJ t a b tRefl => tstar t
-  | tJ t a b p => tJ (tstar t) (tstar a) (tstar b) (tstar p)
-  | tLet (tPack a b) c => (tstar c)[(tstar b) .: (tstar a)..]
-  | tLet a b => tLet (tstar a) (tstar b)
-  | tSig A B => tSig (tstar A) (tstar B)
-  | tPack a b => tPack (tstar a) (tstar b)
+  (* | tZero => tZero *)
+  (* | tSuc a => tSuc (tstar a) *)
+  (* | tInd a b tZero => tstar a *)
+  (* | tInd a b (tSuc c) => (tstar b) [(tInd (tstar a) (tstar b) (tstar c)) .: (tstar c)  .. ] *)
+  (* | tInd a b c => tInd (tstar a) (tstar b) (tstar c) *)
+  (* | tNat => tNat *)
+  (* | tRefl => tRefl *)
+  (* | tEq a b A => tEq (tstar a) (tstar b) (tstar A) *)
+  (* | tJ t a b tRefl => tstar t *)
+  (* | tJ t a b p => tJ (tstar t) (tstar a) (tstar b) (tstar p) *)
+  (* | tLet (tPack a b) c => (tstar c)[(tstar b) .: (tstar a)..] *)
+  (* | tLet a b => tLet (tstar a) (tstar b) *)
+  (* | tSig A B => tSig (tstar A) (tstar B) *)
+                    (* | tPack a b => tPack (tstar a) (tstar b) *)
+  | tVoid => tVoid
+  | tAbsurd a => tAbsurd (tstar a)
   end.
 
 Lemma Par_triangle a : forall b, (a ⇒ b) -> (b ⇒ tstar a).
@@ -556,150 +497,3 @@ Proof.
   case : h => z [*].
   exists z. split; sfirstorder use:@rtc_transitive.
 Qed.
-
-Inductive Sub1 : tm -> tm -> Prop :=
-| Sub_Var n :
-  Sub1 (var_tm n) (var_tm n)
-| Sub_Abs b :
-  Sub1 (tAbs b) (tAbs b)
-| Sub_App b a :
-  Sub1 (tApp b a) (tApp b a)
-| Sub_Zero :
-  Sub1 tZero tZero
-| Sub_Suc a :
-  Sub1 (tSuc a) (tSuc a)
-| Sub_Nat :
-  Sub1 tNat tNat
-| Sub_Ind a b c:
-  Sub1 (tInd a b c) (tInd a b c)
-| Sub_Eq a b A :
-  Sub1 (tEq a b A) (tEq a b A)
-| Sub_J t a b p :
-  Sub1 (tJ t a b p) (tJ t a b p)
-| Sub_Refl :
-  Sub1 tRefl tRefl
-| Sub_Univ i j :
-  i <= j ->
-  Sub1 (tUniv i) (tUniv j)
-| Sub_Prod A0 B0 A1 B1 :
-  Sub1 A1 A0 ->
-  Sub1 B0 B1 ->
-  Sub1 (tPi A0 B0) (tPi A1 B1)
-| Sub_Sig A0 B0 A1 B1 :
-  Sub1 A0 A1 ->
-  Sub1 B0 B1 ->
-  Sub1 (tSig A0 B0) (tSig A1 B1)
-| Sub_Pack a b :
-  Sub1 (tPack a b) (tPack a b)
-| Sub_Let a b :
-  Sub1 (tLet a b) (tLet a b).
-
-Lemma Sub1_refl A : Sub1 A A.
-Proof. elim : A; hauto ctrs:Sub1 solve+:lia. Qed.
-
-Lemma Sub1_transitive A B : Sub1 A B -> forall C, (Sub1 C A -> Sub1 C B) /\ (Sub1 B C -> Sub1 A C).
-Proof.
-  move => h. elim : A B / h; hauto lq:on inv:Sub1 ctrs:Sub1 solve+:lia.
-Qed.
-
-Definition Sub A B :=
-  exists A0 B0, A ⇒* A0 /\ B ⇒* B0 /\ Sub1 A0 B0.
-
-Notation "A <: B" := (Sub A B)  (at level 70, no associativity).
-
-Lemma Sub_reflexive A : Sub A A.
-Proof. hauto lq:on ctrs:rtc use: Sub1_refl unfold:Sub. Qed.
-
-Lemma Sub1_morphing A B (h : Sub1 A B) : forall ρ, Sub1 A[ρ] B[ρ].
-Proof. elim : A B /h; hauto lq:on ctrs:Sub1 use:Sub1_refl solve+:lia. Qed.
-
-Lemma Sub_morphing A B (h : Sub A B) : forall ρ, Sub A[ρ] B[ρ].
-Proof. hauto lq:on use:Par_subst_star, Sub1_morphing unfold:Sub. Qed.
-
-Derive Inversion sub1_inv with (forall A B, Sub1 A B).
-
-Lemma Sub1_simulation A0 A1 (h : A0 ⇒ A1) : forall B0, (Sub1 A0 B0 -> exists B1, Sub1 A1 B1 /\ B0 ⇒ B1) /\ (Sub1 B0 A0 -> exists B1, Sub1 B1 A1 /\ B0 ⇒ B1).
-Proof.
-  elim : A0 A1 /h;
-    match goal with
-    | [|-context[tPi]] =>hauto lq:on rew:off ctrs:Sub1,Par inv:Sub1
-    | [|-context[tSig]] =>hauto lq:on rew:off ctrs:Sub1,Par inv:Sub1
-    | _ => hauto lq:on ctrs:Sub1, Par use:Sub1_refl inv:Sub1
-    end.
-Qed.
-
-Lemma Sub1_simulation_reds A0 A1 (h : A0 ⇒* A1) : forall B0, (Sub1 A0 B0 -> exists B1, Sub1 A1 B1 /\ B0 ⇒* B1) /\ (Sub1 B0 A0 -> exists B1, Sub1 B1 A1 /\ B0 ⇒* B1).
-Proof.
-  elim : A0 A1 /h.
-  - sfirstorder.
-  - move => A0 A1 A2 hr0 hr1 ih B0.
-    split => hB0.
-    + move : Sub1_simulation hr0 hB0. repeat move/[apply].
-      move /(_ B0) => [+ _]. move/[apply]. hauto lq:on rew:off ctrs:rtc.
-    + move : Sub1_simulation hr0 hB0. repeat move/[apply].
-      move /(_ B0) => [_]. move/[apply]. hauto lq:on rew:off ctrs:rtc.
-Qed.
-
-Lemma Sub_transitive A B C : Sub A B -> Sub B C -> Sub A C.
-Proof.
-  rewrite /Sub.
-  move => [A0][B0][h0][h1]h2[B1][C0][h3][h4]h5.
-  have [B'[? ?]] : exists B', B0 ⇒* B' /\ B1 ⇒* B' by sfirstorder use:Pars_confluent.
-  have [A' [??]] : exists A',Sub1 A' B' /\ A0 ⇒* A' by hauto l:on use:Sub1_simulation_reds.
-  have [C' [??]] : exists C',Sub1 B' C' /\ C0 ⇒* C' by hauto l:on use:Sub1_simulation_reds.
-  exists A', C'. repeat split=>//; last by hauto lq:on use:Sub1_transitive.
-  all : eauto using rtc_transitive.
-Qed.
-
-Lemma Sub_univ_inj i j : tUniv i <: tUniv j -> i <= j.
-Proof.
-  rewrite /Sub.
-  move => [A0][B0][+[]].
-  move /Pars_univ_inv => ? /Pars_univ_inv ?. subst.
-  by inversion 1.
-Qed.
-
-Lemma Sub_pi_inj A B A0 B0 : tPi A B <: tPi A0 B0 ->
-  A0 <: A /\ B <: B0.
-Proof.
-  rewrite /Sub.
-  move => [?][?][/Pars_pi_inv].
-  move => [A'][B'][?][? ?]. subst.
-  move =>[/Pars_pi_inv].
-  move => [A''][B''][?][? ?]. subst.
-  hauto lq:on ctrs:Sub1 inv:Sub1.
-Qed.
-
-Lemma Sub_eq_inj a b A a0 b0 A0 (h : Sub (tEq a b A) (tEq a0 b0 A0)) : Coherent a a0 /\ Coherent b b0 /\ Coherent A A0.
-Proof.
-  move : h. rewrite /Sub.
-  move => [A1][A2][/Pars_eq_inv h0][/Pars_eq_inv h1]h2.
-  rewrite /Coherent.
-  hauto lq:on rew:off inv:Sub1.
-Qed.
-
-Lemma Sub_sig_inj A B A0 B0 : Sub (tSig A B) (tSig A0 B0) ->
-  A <: A0 /\ B <: B0.
-Proof.
-  rewrite /Sub.
-  move => [?][?][/Pars_sig_inv].
-  move => [A'][B'][->][? ?].
-  move => [/Pars_sig_inv].
-  move => [A''][B''][->][? ?].
-  hauto lq:on inv:Sub1.
-Qed.
-
-Lemma Sub_renaming A B : forall ξ, A <: B -> A⟨ξ⟩ <: B⟨ξ⟩.
-Proof. move => ξ + /ltac:(substify). move /Sub_morphing. by apply. Qed.
-
-Lemma Sub1_Sub A B : Sub1 A B -> Sub A B.
-Proof. sfirstorder ctrs:rtc unfold:Sub. Qed.
-
-Lemma Par_Sub a b :
-  a ⇒ b -> a <: b /\ b <: a.
-Proof.
-  hauto lq:on use:Sub1_refl ctrs:rtc unfold:Sub.
-Qed.
-
-Lemma Coherent_Sub a b : a ⇔ b -> a <: b.
-Proof. sfirstorder use:Sub1_refl unfold:Coherent, Sub. Qed.
